theories/Dot/unary_lr_binding.v
@@ -3,24 +3,12 @@ From D.Dot Require Export unary_lr synLemmas.
 Import uPred.
 
 Implicit Types
-         (L T U: ty) (v: vl) (e: tm) (d: dm) (ds: dms)
+         (L T U: ty) (v: vl) (e: tm)
          (Γ : ctx) (ρ : vls).
 
 (* Lemmas about the logical relation itself. *)
 Section logrel_binding_lemmas.
   Context `{!dlangG Σ}.
-
-  Lemma def_interp_v_closed T d ρ: (def_interp T ρ d → ⌜ nclosed d 0 ⌝)%I.
-  Proof.
-    iInduction T as [] "IH" forall (ρ d); iIntros "#HT //="; by iDestruct "HT" as "[% _]".
-  Qed.
-
-  Lemma defs_interp_v_closed T ds ρ: defs_interp T ρ ds -∗ ⌜ nclosed ds 0 ⌝%I.
-  Proof.
-    iInduction T as [] "IH" forall (ρ ds);
-      iIntros "#HT //="; try iDestruct "HT" as (l1 d) "[% ?]"; ev; trivial.
-    iDestruct "HT" as "[HT1 _]"; by iApply "IH".
-  Qed.
 
   Lemma interp_weaken ρ1 ρ2 ρ3 τ :
     ⟦ τ.|[upn (length ρ1) (ren (+ length ρ2))] ⟧ (ρ1 ++ ρ2 ++ ρ3)
